{\scriptsize
The equation system is:
\begin{align*}
2x^{2}+x-y^{2}-5&= 0, &&(1)\\
x^{2}-2y^{2}+y-1&= 0. &&(2)\\
\end{align*}
Eliminating leading terms of (1) and (2):
\begin{align*}
2x^{2}+x-y^{2}-5&\underset{(2)}{\rightarrow}\frac{1}{2}x+\frac{3}{2}y^{2}-y-\frac{3}{2}
\sim \\ &\qquad x+3y^{2}-2y-3
.\\ \end{align*}
Equation added:
\begin{align*}
x+3y^{2}-2y-3&= 0. &&(3)\\
\end{align*}
Eliminating leading terms of (1) and (3):
\begin{align*}
2x^{2}+x-y^{2}-5&\underset{(3)}{\rightarrow}-3xy^{2}+2xy+\frac{7}{2}x-\frac{1}{2}y^{2}-\frac{5}{2}
\\ &\underset{(3)}{\rightarrow}-\frac{2}{3}xy-\frac{7}{6}x-3y^{4}+2y^{3}+\frac{19}{6}y^{2}+\frac{5}{6}
\\ &\underset{(3)}{\rightarrow}\frac{7}{4}x+\frac{9}{2}y^{4}-6y^{3}-\frac{11}{4}y^{2}+3y-\frac{5}{4}
\\ &\underset{(3)}{\rightarrow}\frac{18}{7}y^{4}-\frac{24}{7}y^{3}-\frac{32}{7}y^{2}+\frac{26}{7}y+\frac{16}{7}
\sim \\ &\qquad y^{4}-\frac{4}{3}y^{3}-\frac{16}{9}y^{2}+\frac{13}{9}y+\frac{8}{9}
.\\ \end{align*}
Equation added:
\begin{align*}
y^{4}-\frac{4}{3}y^{3}-\frac{16}{9}y^{2}+\frac{13}{9}y+\frac{8}{9}&= 0. &&(4)\\
\end{align*}
Eliminating leading terms of (2) and (3):
\begin{align*}
x^{2}-2y^{2}+y-1&\underset{(3)}{\rightarrow}-3xy^{2}+2xy+3x-2y^{2}+y-1
\\ &\underset{(3)}{\rightarrow}-\frac{2}{3}xy-x-3y^{4}+2y^{3}+\frac{11}{3}y^{2}-\frac{1}{3}y+\frac{1}{3}
\\ &\underset{(3)}{\rightarrow}\frac{3}{2}x+\frac{9}{2}y^{4}-6y^{3}-\frac{7}{2}y^{2}+\frac{7}{2}y-\frac{1}{2}
\\ &\underset{(3)}{\rightarrow}3y^{4}-4y^{3}-\frac{16}{3}y^{2}+\frac{13}{3}y+\frac{8}{3}
\\ &\underset{(4)}{\rightarrow}0
.\\ \end{align*}
Eliminating leading terms of (1) and (4):
\begin{align*}
2x^{2}+x-y^{2}-5&\underset{(4)}{\rightarrow}\frac{4}{3}x^{2}y^{3}+\frac{16}{9}x^{2}y^{2}-\frac{13}{9}x^{2}y-\frac{8}{9}x^{2}+\frac{1}{2}xy^{4}-\frac{1}{2}y^{6}-\frac{5}{2}y^{4}
\\ &\underset{(1)}{\rightarrow}\frac{4}{3}x^{2}y^{2}-\frac{13}{12}x^{2}y-\frac{2}{3}x^{2}+\frac{3}{8}xy^{4}-\frac{1}{2}xy^{3}-\frac{3}{8}y^{6}+\frac{1}{2}y^{5}-\frac{15}{8}y^{4}+\frac{5}{2}y^{3}
\\ &\underset{(1)}{\rightarrow}-\frac{13}{16}x^{2}y-\frac{1}{2}x^{2}+\frac{9}{32}xy^{4}-\frac{3}{8}xy^{3}-\frac{1}{2}xy^{2}-\frac{9}{32}y^{6}+\frac{3}{8}y^{5}-\frac{29}{32}y^{4}+\frac{15}{8}y^{3}+\frac{5}{2}y^{2}
\\ &\underset{(1)}{\rightarrow}\frac{8}{13}x^{2}-\frac{9}{26}xy^{4}+\frac{6}{13}xy^{3}+\frac{8}{13}xy^{2}-\frac{1}{2}xy+\frac{9}{26}y^{6}-\frac{6}{13}y^{5}+\frac{29}{26}y^{4}-\frac{47}{26}y^{3}-\frac{40}{13}y^{2}+\frac{5}{2}y
\\ &\underset{(1)}{\rightarrow}-\frac{9}{16}xy^{4}+\frac{3}{4}xy^{3}+xy^{2}-\frac{13}{16}xy-\frac{1}{2}x+\frac{9}{16}y^{6}-\frac{3}{4}y^{5}+\frac{29}{16}y^{4}-\frac{47}{16}y^{3}-\frac{9}{2}y^{2}+\frac{65}{16}y+\frac{5}{2}
\\ &\underset{(3)}{\rightarrow}-\frac{4}{3}xy^{3}-\frac{16}{9}xy^{2}+\frac{13}{9}xy+\frac{8}{9}x-4y^{6}+\frac{10}{3}y^{5}-\frac{2}{9}y^{4}+\frac{47}{9}y^{3}+8y^{2}-\frac{65}{9}y-\frac{40}{9}
\\ &\underset{(3)}{\rightarrow}\frac{4}{3}xy^{2}-\frac{13}{12}xy-\frac{2}{3}x+3y^{6}-\frac{11}{2}y^{5}+\frac{13}{6}y^{4}-\frac{11}{12}y^{3}-6y^{2}+\frac{65}{12}y+\frac{10}{3}
\\ &\underset{(3)}{\rightarrow}-\frac{13}{16}xy-\frac{1}{2}x+\frac{9}{4}y^{6}-\frac{33}{8}y^{5}-\frac{11}{8}y^{4}+\frac{21}{16}y^{3}-\frac{3}{2}y^{2}+\frac{65}{16}y+\frac{5}{2}
\\ &\underset{(3)}{\rightarrow}\frac{8}{13}x-\frac{36}{13}y^{6}+\frac{66}{13}y^{5}+\frac{22}{13}y^{4}-\frac{60}{13}y^{3}+\frac{50}{13}y^{2}-2y-\frac{40}{13}
\\ &\underset{(3)}{\rightarrow}-\frac{9}{2}y^{6}+\frac{33}{4}y^{5}+\frac{11}{4}y^{4}-\frac{15}{2}y^{3}+\frac{13}{4}y^{2}-\frac{5}{4}y-2
\\ &\underset{(4)}{\rightarrow}-\frac{1}{2}y^{5}+\frac{7}{6}y^{4}+\frac{2}{9}y^{3}-\frac{29}{18}y^{2}+\frac{5}{18}y+\frac{4}{9}
\\ &\underset{(4)}{\rightarrow}-y^{4}+\frac{4}{3}y^{3}+\frac{16}{9}y^{2}-\frac{13}{9}y-\frac{8}{9}
\\ &\underset{(4)}{\rightarrow}0
.\\ \end{align*}
Eliminating leading terms of (2) and (4):
\begin{align*}
x^{2}-2y^{2}+y-1&\underset{(4)}{\rightarrow}\frac{4}{3}x^{2}y^{3}+\frac{16}{9}x^{2}y^{2}-\frac{13}{9}x^{2}y-\frac{8}{9}x^{2}-2y^{6}+y^{5}-y^{4}
\\ &\underset{(1)}{\rightarrow}\frac{4}{3}x^{2}y^{2}-\frac{13}{12}x^{2}y-\frac{2}{3}x^{2}-\frac{1}{2}xy^{3}-\frac{3}{2}y^{6}+\frac{5}{4}y^{5}-\frac{3}{4}y^{4}+\frac{5}{2}y^{3}
\\ &\underset{(1)}{\rightarrow}-\frac{13}{16}x^{2}y-\frac{1}{2}x^{2}-\frac{3}{8}xy^{3}-\frac{1}{2}xy^{2}-\frac{9}{8}y^{6}+\frac{15}{16}y^{5}-\frac{1}{16}y^{4}+\frac{15}{8}y^{3}+\frac{5}{2}y^{2}
\\ &\underset{(1)}{\rightarrow}\frac{8}{13}x^{2}+\frac{6}{13}xy^{3}+\frac{8}{13}xy^{2}-\frac{1}{2}xy+\frac{18}{13}y^{6}-\frac{15}{13}y^{5}+\frac{1}{13}y^{4}-\frac{47}{26}y^{3}-\frac{40}{13}y^{2}+\frac{5}{2}y
\\ &\underset{(1)}{\rightarrow}\frac{3}{4}xy^{3}+xy^{2}-\frac{13}{16}xy-\frac{1}{2}x+\frac{9}{4}y^{6}-\frac{15}{8}y^{5}+\frac{1}{8}y^{4}-\frac{47}{16}y^{3}-\frac{9}{2}y^{2}+\frac{65}{16}y+\frac{5}{2}
\\ &\underset{(3)}{\rightarrow}\frac{4}{3}xy^{2}-\frac{13}{12}xy-\frac{2}{3}x+3y^{6}-\frac{11}{2}y^{5}+\frac{13}{6}y^{4}-\frac{11}{12}y^{3}-6y^{2}+\frac{65}{12}y+\frac{10}{3}
\\ &\underset{(3)}{\rightarrow}-\frac{13}{16}xy-\frac{1}{2}x+\frac{9}{4}y^{6}-\frac{33}{8}y^{5}-\frac{11}{8}y^{4}+\frac{21}{16}y^{3}-\frac{3}{2}y^{2}+\frac{65}{16}y+\frac{5}{2}
\\ &\underset{(3)}{\rightarrow}\frac{8}{13}x-\frac{36}{13}y^{6}+\frac{66}{13}y^{5}+\frac{22}{13}y^{4}-\frac{60}{13}y^{3}+\frac{50}{13}y^{2}-2y-\frac{40}{13}
\\ &\underset{(3)}{\rightarrow}-\frac{9}{2}y^{6}+\frac{33}{4}y^{5}+\frac{11}{4}y^{4}-\frac{15}{2}y^{3}+\frac{13}{4}y^{2}-\frac{5}{4}y-2
\\ &\underset{(4)}{\rightarrow}-\frac{1}{2}y^{5}+\frac{7}{6}y^{4}+\frac{2}{9}y^{3}-\frac{29}{18}y^{2}+\frac{5}{18}y+\frac{4}{9}
\\ &\underset{(4)}{\rightarrow}-y^{4}+\frac{4}{3}y^{3}+\frac{16}{9}y^{2}-\frac{13}{9}y-\frac{8}{9}
\\ &\underset{(4)}{\rightarrow}0
.\\ \end{align*}
Eliminating leading terms of (3) and (4):
\begin{align*}
x+3y^{2}-2y-3&\underset{(4)}{\rightarrow}\frac{4}{3}xy^{3}+\frac{16}{9}xy^{2}-\frac{13}{9}xy-\frac{8}{9}x+3y^{6}-2y^{5}-3y^{4}
\\ &\underset{(3)}{\rightarrow}\frac{4}{3}xy^{2}-\frac{13}{12}xy-\frac{2}{3}x+\frac{9}{4}y^{6}-\frac{9}{2}y^{5}-\frac{1}{4}y^{4}+3y^{3}
\\ &\underset{(3)}{\rightarrow}-\frac{13}{16}xy-\frac{1}{2}x+\frac{27}{16}y^{6}-\frac{27}{8}y^{5}-\frac{51}{16}y^{4}+\frac{17}{4}y^{3}+3y^{2}
\\ &\underset{(3)}{\rightarrow}\frac{8}{13}x-\frac{27}{13}y^{6}+\frac{54}{13}y^{5}+\frac{51}{13}y^{4}-\frac{107}{13}y^{3}-\frac{22}{13}y^{2}+3y
\\ &\underset{(3)}{\rightarrow}-\frac{27}{8}y^{6}+\frac{27}{4}y^{5}+\frac{51}{8}y^{4}-\frac{107}{8}y^{3}-\frac{23}{4}y^{2}+\frac{55}{8}y+3
\\ &\underset{(4)}{\rightarrow}-\frac{2}{3}y^{5}-\frac{1}{9}y^{4}+\frac{68}{27}y^{3}+\frac{22}{27}y^{2}-\frac{55}{27}y-\frac{8}{9}
\\ &\underset{(4)}{\rightarrow}\frac{3}{2}y^{4}-2y^{3}-\frac{8}{3}y^{2}+\frac{13}{6}y+\frac{4}{3}
\\ &\underset{(4)}{\rightarrow}0
.\\ \end{align*}
}