{\scriptsize
The equation system is:
\begin{align*}
3a+2b+c-5&= 0, &&(1)\\
2a+3b-4c+2&= 0, &&(2)\\
5a-b+2c-7&= 0. &&(3)\\
\end{align*}
Eliminating leading terms of (2) and (3):
\begin{align*}
2a+3b-4c+2&\underset{(3)}{\rightarrow}\frac{17}{10}b-\frac{12}{5}c+\frac{12}{5}
\sim \\ &\qquad b-\frac{24}{17}c+\frac{24}{17}
.\\ \end{align*}
Equation added:
\begin{align*}
b-\frac{24}{17}c+\frac{24}{17}&= 0. &&(4)\\
\end{align*}
Eliminating leading terms of (3) and (4):
\begin{align*}
5a-b+2c-7&\underset{(4)}{\rightarrow}\frac{24}{17}ac-\frac{24}{17}a-\frac{1}{5}b^{2}+\frac{2}{5}bc-\frac{7}{5}b
\\ &\underset{(1)}{\rightarrow}-a-\frac{17}{120}b^{2}-\frac{23}{60}bc-\frac{119}{120}b-\frac{1}{3}c^{2}+\frac{5}{3}c
\\ &\underset{(1)}{\rightarrow}\frac{17}{120}b^{2}+\frac{23}{60}bc+\frac{13}{40}b+\frac{1}{3}c^{2}-2c+\frac{5}{3}
\\ &\underset{(4)}{\rightarrow}\frac{70}{17}bc+\frac{15}{17}b+\frac{40}{17}c^{2}-\frac{240}{17}c+\frac{200}{17}
\\ &\underset{(4)}{\rightarrow}\frac{3}{14}b+\frac{236}{119}c^{2}-\frac{576}{119}c+\frac{20}{7}
\\ &\underset{(4)}{\rightarrow}\frac{472}{51}c^{2}-\frac{360}{17}c+\frac{608}{51}
\sim \\ &\qquad c^{2}-\frac{135}{59}c+\frac{76}{59}
.\\ \end{align*}
Equation added:
\begin{align*}
c^{2}-\frac{135}{59}c+\frac{76}{59}&= 0. &&(5)\\
\end{align*}
Eliminating leading terms of (4) and (5):
\begin{align*}
b-\frac{24}{17}c+\frac{24}{17}&\underset{(5)}{\rightarrow}\frac{135}{59}bc-\frac{76}{59}b-\frac{24}{17}c^{3}+\frac{24}{17}c^{2}
\\ &\underset{(4)}{\rightarrow}-\frac{76}{135}b-\frac{472}{765}c^{3}+\frac{1552}{765}c^{2}-\frac{24}{17}c
\\ &\underset{(4)}{\rightarrow}\frac{354}{323}c^{3}-\frac{1164}{323}c^{2}+\frac{1266}{323}c-\frac{24}{17}
\\ &\underset{(5)}{\rightarrow}-c^{2}+\frac{135}{59}c-\frac{76}{59}
\\ &\underset{(5)}{\rightarrow}0
.\\ \end{align*}
Eliminating leading terms of (3) and (5):
\begin{align*}
5a-b+2c-7&\underset{(5)}{\rightarrow}\frac{135}{59}ac-\frac{76}{59}a-\frac{1}{5}bc^{2}+\frac{2}{5}c^{3}-\frac{7}{5}c^{2}
\\ &\underset{(1)}{\rightarrow}-\frac{76}{135}a-\frac{59}{675}bc^{2}-\frac{2}{3}bc+\frac{118}{675}c^{3}-\frac{638}{675}c^{2}+\frac{5}{3}c
\\ &\underset{(1)}{\rightarrow}\frac{59}{380}bc^{2}+\frac{45}{38}bc-\frac{2}{3}b-\frac{59}{190}c^{3}+\frac{319}{190}c^{2}-\frac{751}{228}c+\frac{5}{3}
\\ &\underset{(4)}{\rightarrow}\frac{450}{59}bc-\frac{760}{177}b-\frac{10}{17}c^{3}+\frac{9430}{1003}c^{2}-\frac{3755}{177}c+\frac{1900}{177}
\\ &\underset{(4)}{\rightarrow}-\frac{76}{135}b-\frac{59}{765}c^{3}+\frac{119}{45}c^{2}-\frac{19247}{4590}c+\frac{38}{27}
\\ &\underset{(4)}{\rightarrow}\frac{177}{1292}c^{3}-\frac{357}{76}c^{2}+\frac{1205}{136}c-\frac{133}{34}
\\ &\underset{(5)}{\rightarrow}-32c^{2}+\frac{22439}{354}c-\frac{5054}{177}
\\ &\underset{(5)}{\rightarrow}\frac{59}{192}c-\frac{19}{48}
\sim \\ &\qquad c-\frac{76}{59}
.\\ \end{align*}
Equation added:
\begin{align*}
c-\frac{76}{59}&= 0. &&(6)\\
\end{align*}
Eliminating leading terms of (5) and (6):
\begin{align*}
c^{2}-\frac{135}{59}c+\frac{76}{59}&\underset{(6)}{\rightarrow}-c+\frac{76}{59}
\\ &\underset{(6)}{\rightarrow}0
.\\ \end{align*}
Eliminating leading terms of (4) and (6):
\begin{align*}
b-\frac{24}{17}c+\frac{24}{17}&\underset{(6)}{\rightarrow}\frac{76}{59}b-\frac{24}{17}c^{2}+\frac{24}{17}c
\\ &\underset{(4)}{\rightarrow}-\frac{354}{323}c^{2}+\frac{810}{323}c-\frac{24}{17}
\\ &\underset{(5)}{\rightarrow}0
.\\ \end{align*}
Eliminating leading terms of (3) and (6):
\begin{align*}
5a-b+2c-7&\underset{(6)}{\rightarrow}\frac{76}{59}a-\frac{1}{5}bc+\frac{2}{5}c^{2}-\frac{7}{5}c
\\ &\underset{(1)}{\rightarrow}-\frac{59}{380}bc-\frac{2}{3}b+\frac{59}{190}c^{2}-\frac{1619}{1140}c+\frac{5}{3}
\\ &\underset{(4)}{\rightarrow}\frac{760}{177}b-\frac{10}{17}c^{2}+\frac{23275}{3009}c-\frac{1900}{177}
\\ &\underset{(4)}{\rightarrow}-\frac{177}{1292}c^{2}+\frac{437}{136}c-\frac{133}{34}
\\ &\underset{(5)}{\rightarrow}-\frac{127}{6}c+\frac{4826}{177}
\\ &\underset{(6)}{\rightarrow}0
.\\ \end{align*}
Eliminating leading terms of (2) and (6):
\begin{align*}
2a+3b-4c+2&\underset{(6)}{\rightarrow}\frac{76}{59}a+\frac{3}{2}bc-2c^{2}+c
\\ &\underset{(1)}{\rightarrow}\frac{177}{152}bc-\frac{2}{3}b-\frac{59}{38}c^{2}+\frac{101}{228}c+\frac{5}{3}
\\ &\underset{(4)}{\rightarrow}-\frac{304}{531}b+\frac{4}{51}c^{2}-\frac{9310}{9027}c+\frac{760}{531}
\\ &\underset{(4)}{\rightarrow}-\frac{177}{1292}c^{2}+\frac{437}{136}c-\frac{133}{34}
\\ &\underset{(5)}{\rightarrow}-\frac{127}{6}c+\frac{4826}{177}
\\ &\underset{(6)}{\rightarrow}0
.\\ \end{align*}
Eliminating leading terms of (1) and (6):
\begin{align*}
3a+2b+c-5&\underset{(6)}{\rightarrow}\frac{76}{59}a+\frac{2}{3}bc+\frac{1}{3}c^{2}-\frac{5}{3}c
\\ &\underset{(1)}{\rightarrow}\frac{59}{114}bc-\frac{2}{3}b+\frac{59}{228}c^{2}-\frac{371}{228}c+\frac{5}{3}
\\ &\underset{(4)}{\rightarrow}-\frac{76}{59}b+\frac{65}{34}c^{2}-\frac{9139}{2006}c+\frac{190}{59}
\\ &\underset{(4)}{\rightarrow}-\frac{3835}{2584}c^{2}+\frac{673}{136}c-\frac{133}{34}
\\ &\underset{(5)}{\rightarrow}-\frac{68}{65}c+\frac{5168}{3835}
\\ &\underset{(6)}{\rightarrow}0
.\\ \end{align*}
Eliminating leading terms of (2) and (5):
\begin{align*}
2a+3b-4c+2&\underset{(5)}{\rightarrow}\frac{135}{59}ac-\frac{76}{59}a+\frac{3}{2}bc^{2}-2c^{3}+c^{2}
\\ &\underset{(1)}{\rightarrow}-\frac{76}{135}a+\frac{59}{90}bc^{2}-\frac{2}{3}bc-\frac{118}{135}c^{3}+\frac{14}{135}c^{2}+\frac{5}{3}c
\\ &\underset{(1)}{\rightarrow}-\frac{177}{152}bc^{2}+\frac{45}{38}bc-\frac{2}{3}b+\frac{59}{38}c^{3}-\frac{7}{38}c^{2}-\frac{751}{228}c+\frac{5}{3}
\\ &\underset{(4)}{\rightarrow}-\frac{60}{59}bc+\frac{304}{531}b+\frac{4}{51}c^{3}-\frac{3772}{3009}c^{2}+\frac{1502}{531}c-\frac{760}{531}
\\ &\underset{(4)}{\rightarrow}-\frac{76}{135}b-\frac{59}{765}c^{3}+\frac{119}{45}c^{2}-\frac{19247}{4590}c+\frac{38}{27}
\\ &\underset{(4)}{\rightarrow}\frac{177}{1292}c^{3}-\frac{357}{76}c^{2}+\frac{1205}{136}c-\frac{133}{34}
\\ &\underset{(5)}{\rightarrow}-32c^{2}+\frac{22439}{354}c-\frac{5054}{177}
\\ &\underset{(5)}{\rightarrow}\frac{59}{192}c-\frac{19}{48}
\\ &\underset{(6)}{\rightarrow}0
.\\ \end{align*}
Eliminating leading terms of (1) and (5):
\begin{align*}
3a+2b+c-5&\underset{(5)}{\rightarrow}\frac{135}{59}ac-\frac{76}{59}a+\frac{2}{3}bc^{2}+\frac{1}{3}c^{3}-\frac{5}{3}c^{2}
\\ &\underset{(1)}{\rightarrow}-\frac{76}{135}a+\frac{118}{405}bc^{2}-\frac{2}{3}bc+\frac{59}{405}c^{3}-\frac{86}{81}c^{2}+\frac{5}{3}c
\\ &\underset{(1)}{\rightarrow}-\frac{59}{114}bc^{2}+\frac{45}{38}bc-\frac{2}{3}b-\frac{59}{228}c^{3}+\frac{215}{114}c^{2}-\frac{751}{228}c+\frac{5}{3}
\\ &\underset{(4)}{\rightarrow}-\frac{135}{59}bc+\frac{76}{59}b+\frac{65}{34}c^{3}-\frac{5071}{1003}c^{2}+\frac{751}{118}c-\frac{190}{59}
\\ &\underset{(4)}{\rightarrow}-\frac{76}{135}b-\frac{767}{918}c^{3}+\frac{8311}{2295}c^{2}-\frac{19247}{4590}c+\frac{38}{27}
\\ &\underset{(4)}{\rightarrow}\frac{3835}{2584}c^{3}-\frac{8311}{1292}c^{2}+\frac{1205}{136}c-\frac{133}{34}
\\ &\underset{(5)}{\rightarrow}-\frac{133}{65}c^{2}+\frac{3591}{767}c-\frac{10108}{3835}
\\ &\underset{(5)}{\rightarrow}0
.\\ \end{align*}
Eliminating leading terms of (2) and (4):
\begin{align*}
2a+3b-4c+2&\underset{(4)}{\rightarrow}\frac{24}{17}ac-\frac{24}{17}a+\frac{3}{2}b^{2}-2bc+b
\\ &\underset{(1)}{\rightarrow}-a+\frac{17}{16}b^{2}-\frac{25}{12}bc+\frac{17}{24}b-\frac{1}{3}c^{2}+\frac{5}{3}c
\\ &\underset{(1)}{\rightarrow}-\frac{17}{16}b^{2}+\frac{25}{12}bc-\frac{11}{8}b+\frac{1}{3}c^{2}-2c+\frac{5}{3}
\\ &\underset{(4)}{\rightarrow}-\frac{28}{51}bc-\frac{2}{17}b-\frac{16}{51}c^{2}+\frac{32}{17}c-\frac{80}{51}
\\ &\underset{(4)}{\rightarrow}\frac{3}{14}b+\frac{236}{119}c^{2}-\frac{576}{119}c+\frac{20}{7}
\\ &\underset{(4)}{\rightarrow}\frac{472}{51}c^{2}-\frac{360}{17}c+\frac{608}{51}
\\ &\underset{(5)}{\rightarrow}0
.\\ \end{align*}
Eliminating leading terms of (1) and (4):
\begin{align*}
3a+2b+c-5&\underset{(4)}{\rightarrow}\frac{24}{17}ac-\frac{24}{17}a+\frac{2}{3}b^{2}+\frac{1}{3}bc-\frac{5}{3}b
\\ &\underset{(1)}{\rightarrow}-a+\frac{17}{36}b^{2}-\frac{31}{72}bc-\frac{85}{72}b-\frac{1}{3}c^{2}+\frac{5}{3}c
\\ &\underset{(1)}{\rightarrow}-\frac{17}{36}b^{2}+\frac{31}{72}bc+\frac{37}{72}b+\frac{1}{3}c^{2}-2c+\frac{5}{3}
\\ &\underset{(4)}{\rightarrow}\frac{1}{2}bc-\frac{5}{2}b-\frac{12}{17}c^{2}+\frac{72}{17}c-\frac{60}{17}
\\ &\underset{(4)}{\rightarrow}-5b+\frac{120}{17}c-\frac{120}{17}
\\ &\underset{(4)}{\rightarrow}0
.\\ \end{align*}
Eliminating leading terms of (1) and (3):
\begin{align*}
3a+2b+c-5&\underset{(3)}{\rightarrow}\frac{13}{15}b-\frac{1}{15}c-\frac{4}{15}
\\ &\underset{(4)}{\rightarrow}\frac{295}{221}c-\frac{380}{221}
\\ &\underset{(6)}{\rightarrow}0
.\\ \end{align*}
Eliminating leading terms of (1) and (2):
\begin{align*}
3a+2b+c-5&\underset{(2)}{\rightarrow}-\frac{5}{6}b+\frac{7}{3}c-\frac{8}{3}
\\ &\underset{(4)}{\rightarrow}-\frac{118}{85}c+\frac{152}{85}
\\ &\underset{(6)}{\rightarrow}0
.\\ \end{align*}
}
