{\scriptsize
The equation system is:
\begin{align*}
3a+2b+c-5&= 0, &&(1)\\
2a+3b-4c+2&= 0, &&(2)\\
5a-b+2c-7&= 0. &&(3)\\
\end{align*}
Eliminating leading terms of (1) and (2):
\begin{align*}
3a+2b+c-5&\underset{(2)}{\rightarrow}-\frac{5}{6}b+\frac{7}{3}c-\frac{8}{3}
\sim \\ &\qquad b-\frac{14}{5}c+\frac{16}{5}
.\\ \end{align*}
Equation added:
\begin{align*}
b-\frac{14}{5}c+\frac{16}{5}&= 0. &&(4)\\
\end{align*}
Eliminating leading terms of (1) and (3):
\begin{align*}
3a+2b+c-5&\underset{(3)}{\rightarrow}\frac{13}{15}b-\frac{1}{15}c-\frac{4}{15}
\\ &\underset{(4)}{\rightarrow}\frac{177}{65}c-\frac{228}{65}
\sim \\ &\qquad c-\frac{76}{59}
.\\ \end{align*}
Equation added:
\begin{align*}
c-\frac{76}{59}&= 0. &&(5)\\
\end{align*}
Eliminating leading terms of (2) and (3):
\begin{align*}
2a+3b-4c+2&\underset{(3)}{\rightarrow}\frac{17}{10}b-\frac{12}{5}c+\frac{12}{5}
\\ &\underset{(4)}{\rightarrow}\frac{118}{85}c-\frac{152}{85}
\\ &\underset{(5)}{\rightarrow}0
.\\ \end{align*}
Eliminating leading terms of (1) and (4):
\begin{align*}
3a+2b+c-5&\underset{(4)}{\rightarrow}\frac{14}{5}ac-\frac{16}{5}a+\frac{2}{3}b^{2}+\frac{1}{3}bc-\frac{5}{3}b
\\ &\underset{(5)}{\rightarrow}\frac{60}{413}a+\frac{5}{21}b^{2}+\frac{5}{42}bc-\frac{25}{42}b
\\ &\underset{(3)}{\rightarrow}\frac{59}{36}b^{2}+\frac{59}{72}bc-\frac{1403}{360}b-\frac{2}{5}c+\frac{7}{5}
\\ &\underset{(4)}{\rightarrow}\frac{33}{10}bc-\frac{3291}{590}b-\frac{72}{295}c+\frac{252}{295}
\\ &\underset{(5)}{\rightarrow}-\frac{261}{649}b-\frac{48}{649}c+\frac{168}{649}
\\ &\underset{(4)}{\rightarrow}\frac{1298}{435}c-\frac{1672}{435}
\\ &\underset{(5)}{\rightarrow}0
.\\ \end{align*}
Eliminating leading terms of (2) and (4):
\begin{align*}
2a+3b-4c+2&\underset{(4)}{\rightarrow}\frac{14}{5}ac-\frac{16}{5}a+\frac{3}{2}b^{2}-2bc+b
\\ &\underset{(5)}{\rightarrow}\frac{60}{413}a+\frac{15}{28}b^{2}-\frac{5}{7}bc+\frac{5}{14}b
\\ &\underset{(3)}{\rightarrow}\frac{59}{16}b^{2}-\frac{59}{12}bc+\frac{319}{120}b-\frac{2}{5}c+\frac{7}{5}
\\ &\underset{(4)}{\rightarrow}\frac{22}{15}bc-\frac{2194}{885}b-\frac{32}{295}c+\frac{112}{295}
\\ &\underset{(5)}{\rightarrow}-\frac{261}{649}b-\frac{48}{649}c+\frac{168}{649}
\\ &\underset{(4)}{\rightarrow}\frac{1298}{435}c-\frac{1672}{435}
\\ &\underset{(5)}{\rightarrow}0
.\\ \end{align*}
Eliminating leading terms of (3) and (4):
\begin{align*}
5a-b+2c-7&\underset{(4)}{\rightarrow}\frac{14}{5}ac-\frac{16}{5}a-\frac{1}{5}b^{2}+\frac{2}{5}bc-\frac{7}{5}b
\\ &\underset{(5)}{\rightarrow}\frac{60}{413}a-\frac{1}{14}b^{2}+\frac{1}{7}bc-\frac{1}{2}b
\\ &\underset{(3)}{\rightarrow}-\frac{59}{120}b^{2}+\frac{59}{60}bc-\frac{389}{120}b-\frac{2}{5}c+\frac{7}{5}
\\ &\underset{(4)}{\rightarrow}\frac{4}{5}bc+\frac{1001}{295}b+\frac{48}{59}c-\frac{168}{59}
\\ &\underset{(5)}{\rightarrow}\frac{1305}{236}b+\frac{60}{59}c-\frac{210}{59}
\\ &\underset{(4)}{\rightarrow}\frac{1298}{435}c-\frac{1672}{435}
\\ &\underset{(5)}{\rightarrow}0
.\\ \end{align*}
Eliminating leading terms of (1) and (5):
\begin{align*}
3a+2b+c-5&\underset{(5)}{\rightarrow}\frac{76}{59}a+\frac{2}{3}bc+\frac{1}{3}c^{2}-\frac{5}{3}c
\\ &\underset{(3)}{\rightarrow}\frac{59}{114}bc+\frac{1}{5}b+\frac{59}{228}c^{2}-\frac{1931}{1140}c+\frac{7}{5}
\\ &\underset{(5)}{\rightarrow}\frac{494}{295}b+\frac{1}{2}c^{2}-\frac{1931}{590}c+\frac{798}{295}
\\ &\underset{(4)}{\rightarrow}\frac{295}{988}c^{2}+\frac{4177}{4940}c-\frac{103}{65}
\\ &\underset{(5)}{\rightarrow}\frac{103}{25}c-\frac{7828}{1475}
\\ &\underset{(5)}{\rightarrow}0
.\\ \end{align*}
Eliminating leading terms of (2) and (5):
\begin{align*}
2a+3b-4c+2&\underset{(5)}{\rightarrow}\frac{76}{59}a+\frac{3}{2}bc-2c^{2}+c
\\ &\underset{(3)}{\rightarrow}\frac{177}{152}bc+\frac{1}{5}b-\frac{59}{38}c^{2}+\frac{143}{380}c+\frac{7}{5}
\\ &\underset{(5)}{\rightarrow}\frac{1292}{885}b-\frac{4}{3}c^{2}+\frac{286}{885}c+\frac{1064}{885}
\\ &\underset{(4)}{\rightarrow}-\frac{295}{323}c^{2}+\frac{9759}{3230}c-\frac{202}{85}
\\ &\underset{(5)}{\rightarrow}-\frac{101}{50}c+\frac{3838}{1475}
\\ &\underset{(5)}{\rightarrow}0
.\\ \end{align*}
Eliminating leading terms of (3) and (5):
\begin{align*}
5a-b+2c-7&\underset{(5)}{\rightarrow}\frac{76}{59}a-\frac{1}{5}bc+\frac{2}{5}c^{2}-\frac{7}{5}c
\\ &\underset{(3)}{\rightarrow}-\frac{59}{380}bc+\frac{1}{5}b+\frac{59}{190}c^{2}-\frac{113}{76}c+\frac{7}{5}
\\ &\underset{(5)}{\rightarrow}-2c^{2}+\frac{565}{59}c-\frac{532}{59}
\\ &\underset{(5)}{\rightarrow}-\frac{7}{2}c+\frac{266}{59}
\\ &\underset{(5)}{\rightarrow}0
.\\ \end{align*}
Eliminating leading terms of (4) and (5):
\begin{align*}
b-\frac{14}{5}c+\frac{16}{5}&\underset{(5)}{\rightarrow}\frac{76}{59}b-\frac{14}{5}c^{2}+\frac{16}{5}c
\\ &\underset{(4)}{\rightarrow}-\frac{413}{190}c^{2}+\frac{502}{95}c-\frac{16}{5}
\\ &\underset{(5)}{\rightarrow}-\frac{8}{7}c+\frac{608}{413}
\\ &\underset{(5)}{\rightarrow}0
.\\ \end{align*}
}