{\scriptsize
The equation system is:
\begin{align*}
3a+2b+c-5&= 0, &&(1)\\
2a+3b-4c+2&= 0, &&(2)\\
5a-b+2c-7&= 0. &&(3)\\
\end{align*}
Eliminating leading terms of (1) and (2):
\begin{align*}
3a+2b+c-5&\underset{(2)}{\rightarrow}-\frac{5}{6}b+\frac{7}{3}c-\frac{8}{3}
\sim \\ &\qquad b-\frac{14}{5}c+\frac{16}{5}
.\\ \end{align*}
Equation added:
\begin{align*}
b-\frac{14}{5}c+\frac{16}{5}&= 0. &&(4)\\
\end{align*}
Eliminating leading terms of (1) and (3):
\begin{align*}
3a+2b+c-5&\underset{(3)}{\rightarrow}\frac{13}{15}b-\frac{1}{15}c-\frac{4}{15}
\\ &\underset{(4)}{\rightarrow}\frac{177}{65}c-\frac{228}{65}
\sim \\ &\qquad c-\frac{76}{59}
.\\ \end{align*}
Equation added:
\begin{align*}
c-\frac{76}{59}&= 0. &&(5)\\
\end{align*}
Eliminating leading terms of (2) and (3):
\begin{align*}
2a+3b-4c+2&\underset{(3)}{\rightarrow}\frac{17}{10}b-\frac{12}{5}c+\frac{12}{5}
\\ &\underset{(4)}{\rightarrow}\frac{118}{85}c-\frac{152}{85}
\\ &\underset{(5)}{\rightarrow}0
.\\ \end{align*}
Eliminating leading terms of (1) and (4):
\begin{align*}
3a+2b+c-5&\underset{(4)}{\rightarrow}\frac{14}{5}ac-\frac{16}{5}a+\frac{2}{3}b^{2}+\frac{1}{3}bc-\frac{5}{3}b
\\ &\underset{(1)}{\rightarrow}-\frac{8}{7}a+\frac{5}{21}b^{2}-\frac{23}{42}bc-\frac{25}{42}b-\frac{1}{3}c^{2}+\frac{5}{3}c
\\ &\underset{(1)}{\rightarrow}-\frac{5}{24}b^{2}+\frac{23}{48}bc-\frac{7}{48}b+\frac{7}{24}c^{2}-\frac{43}{24}c+\frac{5}{3}
\\ &\underset{(4)}{\rightarrow}\frac{1}{2}bc-\frac{5}{2}b-\frac{7}{5}c^{2}+\frac{43}{5}c-8
\\ &\underset{(4)}{\rightarrow}-5b+14c-16
\\ &\underset{(4)}{\rightarrow}0
.\\ \end{align*}
Eliminating leading terms of (2) and (4):
\begin{align*}
2a+3b-4c+2&\underset{(4)}{\rightarrow}\frac{14}{5}ac-\frac{16}{5}a+\frac{3}{2}b^{2}-2bc+b
\\ &\underset{(1)}{\rightarrow}-\frac{8}{7}a+\frac{15}{28}b^{2}-\frac{29}{21}bc+\frac{5}{14}b-\frac{1}{3}c^{2}+\frac{5}{3}c
\\ &\underset{(1)}{\rightarrow}-\frac{15}{32}b^{2}+\frac{29}{24}bc-\frac{47}{48}b+\frac{7}{24}c^{2}-\frac{43}{24}c+\frac{5}{3}
\\ &\underset{(4)}{\rightarrow}\frac{2}{9}bc-\frac{10}{9}b-\frac{28}{45}c^{2}+\frac{172}{45}c-\frac{32}{9}
\\ &\underset{(4)}{\rightarrow}-5b+14c-16
\\ &\underset{(4)}{\rightarrow}0
.\\ \end{align*}
Eliminating leading terms of (3) and (4):
\begin{align*}
5a-b+2c-7&\underset{(4)}{\rightarrow}\frac{14}{5}ac-\frac{16}{5}a-\frac{1}{5}b^{2}+\frac{2}{5}bc-\frac{7}{5}b
\\ &\underset{(1)}{\rightarrow}-\frac{8}{7}a-\frac{1}{14}b^{2}-\frac{11}{21}bc-\frac{1}{2}b-\frac{1}{3}c^{2}+\frac{5}{3}c
\\ &\underset{(1)}{\rightarrow}\frac{1}{16}b^{2}+\frac{11}{24}bc-\frac{11}{48}b+\frac{7}{24}c^{2}-\frac{43}{24}c+\frac{5}{3}
\\ &\underset{(4)}{\rightarrow}\frac{152}{15}bc-\frac{103}{15}b+\frac{14}{3}c^{2}-\frac{86}{3}c+\frac{80}{3}
\\ &\underset{(4)}{\rightarrow}-\frac{103}{152}b+\frac{1239}{380}c^{2}-\frac{2291}{380}c+\frac{50}{19}
\\ &\underset{(4)}{\rightarrow}-\frac{2478}{515}c^{2}+\frac{6024}{515}c-\frac{3648}{515}
\\ &\underset{(5)}{\rightarrow}-\frac{8}{7}c+\frac{608}{413}
\\ &\underset{(5)}{\rightarrow}0
.\\ \end{align*}
Eliminating leading terms of (1) and (5):
\begin{align*}
3a+2b+c-5&\underset{(5)}{\rightarrow}\frac{76}{59}a+\frac{2}{3}bc+\frac{1}{3}c^{2}-\frac{5}{3}c
\\ &\underset{(1)}{\rightarrow}\frac{59}{114}bc-\frac{2}{3}b+\frac{59}{228}c^{2}-\frac{371}{228}c+\frac{5}{3}
\\ &\underset{(4)}{\rightarrow}-\frac{76}{59}b+\frac{33}{10}c^{2}-\frac{3743}{590}c+\frac{190}{59}
\\ &\underset{(4)}{\rightarrow}-\frac{1947}{760}c^{2}+\frac{309}{40}c-\frac{57}{10}
\\ &\underset{(5)}{\rightarrow}-\frac{19}{11}c+\frac{1444}{649}
\\ &\underset{(5)}{\rightarrow}0
.\\ \end{align*}
Eliminating leading terms of (2) and (5):
\begin{align*}
2a+3b-4c+2&\underset{(5)}{\rightarrow}\frac{76}{59}a+\frac{3}{2}bc-2c^{2}+c
\\ &\underset{(1)}{\rightarrow}\frac{177}{152}bc-\frac{2}{3}b-\frac{59}{38}c^{2}+\frac{101}{228}c+\frac{5}{3}
\\ &\underset{(4)}{\rightarrow}-\frac{304}{531}b+\frac{22}{15}c^{2}-\frac{7486}{2655}c+\frac{760}{531}
\\ &\underset{(4)}{\rightarrow}-\frac{1947}{760}c^{2}+\frac{309}{40}c-\frac{57}{10}
\\ &\underset{(5)}{\rightarrow}-\frac{19}{11}c+\frac{1444}{649}
\\ &\underset{(5)}{\rightarrow}0
.\\ \end{align*}
Eliminating leading terms of (3) and (5):
\begin{align*}
5a-b+2c-7&\underset{(5)}{\rightarrow}\frac{76}{59}a-\frac{1}{5}bc+\frac{2}{5}c^{2}-\frac{7}{5}c
\\ &\underset{(1)}{\rightarrow}-\frac{59}{380}bc-\frac{2}{3}b+\frac{59}{190}c^{2}-\frac{1619}{1140}c+\frac{5}{3}
\\ &\underset{(4)}{\rightarrow}\frac{760}{177}b+\frac{4}{5}c^{2}+\frac{5263}{885}c-\frac{1900}{177}
\\ &\underset{(4)}{\rightarrow}\frac{177}{950}c^{2}+\frac{837}{200}c-\frac{57}{10}
\\ &\underset{(5)}{\rightarrow}\frac{95}{4}c-\frac{1805}{59}
\\ &\underset{(5)}{\rightarrow}0
.\\ \end{align*}
Eliminating leading terms of (4) and (5):
\begin{align*}
b-\frac{14}{5}c+\frac{16}{5}&\underset{(5)}{\rightarrow}\frac{76}{59}b-\frac{14}{5}c^{2}+\frac{16}{5}c
\\ &\underset{(4)}{\rightarrow}-\frac{413}{190}c^{2}+\frac{502}{95}c-\frac{16}{5}
\\ &\underset{(5)}{\rightarrow}-\frac{8}{7}c+\frac{608}{413}
\\ &\underset{(5)}{\rightarrow}0
.\\ \end{align*}
}